Hnr.thy
@@ -1,6 +1,6 @@
 theory Hnr 
-  imports Array_Safe Diff_Arr_Safe
-begin
+  imports Base
+begin                       
 
 definition hnr where "hnr \<Gamma> c \<Gamma>' a = <\<Gamma>> c <\<lambda>r. \<Gamma>' a r>\<^sub>t"
 
@@ -13,10 +13,7 @@ abbreviation id_assn where "id_assn a c \<equiv> \<up>(id_rel a c)"
 
 abbreviation array_assn where "array_assn xs xsi \<equiv> xsi \<mapsto>\<^sub>a xs"
 
-named_theorems hnr_rule_raw
-
-named_theorems hnr_rule_arr
-named_theorems hnr_rule_diff_arr
+named_theorems hnr_rule
 
 lemma hnr_return: "hnr \<Gamma> (return x) (\<lambda> x xi. \<Gamma> * id_assn x xi) x"
   unfolding hnr_def id_rel_def
@@ -57,7 +54,7 @@ method keep_drop_simp = (simp only: star_aci)?; rule ent_refl
 method keep_drop = 
   rule keep_drop_init, ((rule keep_drop_step)+; fail), keep_drop_simp, keep_drop_simp
 
-lemma hnr_let[hnr_rule_raw]:
+lemma hnr_let[hnr_rule]:
   assumes 
     "hnr \<Gamma> vi \<Gamma>\<^sub>1 v" 
     "\<And>xi x. hnr (\<Gamma>\<^sub>1 x xi) (fi xi) (\<Gamma>' x xi) (f x)"
@@ -92,50 +89,25 @@ lemma hnr_if':
     "hnr 
       \<Gamma> 
       (if c then ai else bi) 
-      (\<lambda>a r. \<Gamma>\<^sub>a a r * \<up> c \<or>\<^sub>A \<Gamma>\<^sub>b a r * \<up>(\<not>c)) 
+      (\<lambda>a r. \<Gamma>\<^sub>a a r * \<up>c \<or>\<^sub>A \<Gamma>\<^sub>b a r * \<up>(\<not>c)) 
       (if c then a else b)" 
   supply[sep_heap_rules] = assms[THEN hnrD]
   apply(rule hnrI)
   by(sep_auto simp: ent_star_mono)
 
-(* TODO: 
-lemma hnr_tuple: 
-assumes
-  "hnr \<Gamma> ai \<Gamma>\<^sub>a R\<^sub>a a"
-  "hnr \<Gamma> bi \<Gamma>\<^sub>b R\<^sub>b b"
-shows 
-  "hnr 
-    \<Gamma> 
-    (do { a \<leftarrow> ai; b \<leftarrow> bi; return (a, b) })
-    (\<Gamma>\<^sub>a \<and>\<^sub>A \<Gamma>\<^sub>b) 
-    (\<lambda>(a1, a2) (r1, r2). R\<^sub>a a1 r1 \<and>\<^sub>A R\<^sub>b a2 r2) 
-    (a, b)" 
+lemma hnr_if''[hnr_rule]: 
+  assumes
+    "hnr \<Gamma> ai \<Gamma>\<^sub>a a"
+    "hnr \<Gamma> bi \<Gamma>\<^sub>b b"
+  shows 
+    "hnr 
+      \<Gamma> 
+      (if c then ai else bi) 
+      (\<lambda>a r. (\<up>c * \<Gamma>\<^sub>a a r  \<or>\<^sub>A \<up>(\<not>c) * \<Gamma>\<^sub>b a r) * emp) 
+      (if c then a else b)" 
   supply[sep_heap_rules] = assms[THEN hnrD]
   apply(rule hnrI)
-  apply sep_auto
-  apply(rule fi_rule[of "\<Gamma>"])
-  sorry *)
-
-
-lemma hnr_array_nth [hnr_rule_arr]: "
-    hnr
-     (xsi \<mapsto>\<^sub>a xs * id_assn i ii)
-     (array_nth_safe xsi ii) 
-     (\<lambda> r ri. xsi \<mapsto>\<^sub>a xs * id_assn r ri) 
-     (xs ! i)"
-  unfolding id_rel_def
-  apply(rule hnrI)
-  by sep_auto
-
-lemma hnr_array_update [hnr_rule_arr]: "
-    hnr 
-      (xsi \<mapsto>\<^sub>a xs * id_assn i ii * id_assn v vi) 
-      (array_update_safe ii vi xsi) 
-      array_assn
-      (xs [i:= v])"
-  unfolding id_rel_def
-  apply(rule hnrI)
-  by sep_auto
+  by(sep_auto simp: ent_star_mono)
 
 lemma hnr_pass: "hnr (A x xi) (return xi) A x"
   unfolding id_rel_def
@@ -147,14 +119,75 @@ lemma hnr_copy: "hnr (id_assn x xi) (return xi) id_assn x"
   apply(rule hnrI)
   by sep_auto
 
-lemma hnr_copy_diff_arr [hnr_rule_diff_arr]:
-  "hnr (master_assn t * \<up>(t \<turnstile> x \<sim> xi)) (return xi) (\<lambda>x xi. master_assn t * \<up>(t \<turnstile> x \<sim> xi)) x"
+lemma hnr_tuple: 
+  assumes
+    "hnr \<Gamma> (return ai) \<Gamma>\<^sub>a a"
+    "hnr (\<Gamma>\<^sub>a a ai * true) (return bi) (\<Gamma>\<^sub>b a ai) b"
+  shows 
+    "hnr 
+      \<Gamma>
+      (return (ai, bi))
+      (\<lambda>(a, b)(ai, bi). \<Gamma>\<^sub>b a ai b bi)
+      (a, b)"
   apply(rule hnrI)
+  using 
+    assms[THEN hnrD]
+    htriple_return_entails[of \<Gamma> ai "\<lambda>ai. \<Gamma>\<^sub>a a ai * true"] 
+    htriple_return_entails[of "\<Gamma>\<^sub>a a ai * true" bi "\<lambda>bi. \<Gamma>\<^sub>b a ai b bi * true"]
+    ent_trans[of \<Gamma>]
   by sep_auto
 
-lemma hnr_copy_arr [hnr_rule_arr]:
-  "hnr (array_assn x xi) (return xi) array_assn x"
+lemma merge_and_1: "a \<and>\<^sub>A a = a"
+  by auto
+
+
+lemma merge_and_2_3_1: "times_assn_raw (Rep_assn a) (Rep_assn (Abs_assn (\<lambda>h. h \<Turnstile> b \<and> h \<Turnstile> c))) h \<Longrightarrow> 
+      times_assn_raw (Rep_assn a) (Rep_assn b) h \<and> times_assn_raw (Rep_assn a) (Rep_assn c) h"
+  apply(induction "Rep_assn a" "Rep_assn (Abs_assn (\<lambda>h. h \<Turnstile> b \<and> h \<Turnstile> c))" h rule: times_assn_raw.induct)
+  using inf_assn_def mod_and_dist by auto
+
+lemma merge_and_2_3: "a * (b \<and>\<^sub>A c) \<Longrightarrow>\<^sub>A (a * b) \<and>\<^sub>A (a * c)"
+  unfolding inf_assn_def times_assn_def entails_def
+  apply auto
+  by (metis ent_star_mono entails_def inf_assn_def mod_and_dist times_assn_def)
+
+(*lemma merge_and_2_2_1: "h \<Turnstile> Abs_assn (times_assn_raw (Rep_assn a) (Rep_assn b)) \<and>
+             h \<Turnstile> Abs_assn (times_assn_raw (Rep_assn a) (Rep_assn c)) 
+  \<Longrightarrow> times_assn_raw (Rep_assn a) (Rep_assn (Abs_assn (\<lambda>h. h \<Turnstile> b \<and> h \<Turnstile> c))) h"
+  apply(auto simp: Abs_assn_inverse)
+  apply(induction "Rep_assn a" "Rep_assn b" h rule: times_assn_raw.induct)
+  apply auto
+  subgoal for h as1 as1a as2 as2a
+    apply(subst exI[where x = as1])
+     apply(subst exI[where x = "as2a"])
+      apply auto
+    sorry
+  sorry
+
+lemma merge_and_2_2: "(a * b) \<and>\<^sub>A (a * c) \<Longrightarrow>\<^sub>A a * (b \<and>\<^sub>A c)"
+  unfolding inf_assn_def times_assn_def entails_def 
+  apply auto
+  using Abs_assn_inverse merge_and_2_2_1 by force
+
+lemma merge_and_2: "(a * b) \<and>\<^sub>A (a * c) = a * (b \<and>\<^sub>A c)"
+  unfolding inf_assn_def times_assn_def
+  apply(auto simp: Abs_assn_inverse)
+  sorry *)
+
+lemma hnr_tuple_2[hnr_rule]:
+  assumes
+    "hnr \<Gamma> (return ai) \<Gamma>\<^sub>a a"
+    "hnr \<Gamma> (return bi) \<Gamma>\<^sub>b b"
+  shows 
+    "hnr 
+      \<Gamma>
+      (return (ai, bi))
+      (\<lambda>(a, b)(ai, bi). \<Gamma>\<^sub>a a ai * true \<and>\<^sub>A \<Gamma>\<^sub>b b bi * true)
+      (a, b)"
   apply(rule hnrI)
+  using 
+    assms[THEN hnrD]
+  using htriple_return_and[of \<Gamma> ai "\<lambda>ai. \<Gamma>\<^sub>a a ai * true" bi "\<lambda>bi. \<Gamma>\<^sub>b b bi * true"] ent_true_drop(2)
   by sep_auto
 
 lemma hnr_frame:
@@ -166,39 +199,439 @@ lemma hnr_frame:
   apply(rule hnrI)
   by (smt (verit) assms(1) assms(2) assn_aci(10) fi_rule hnrD hoare_triple_def)
 
-lemma hnr_lookup[hnr_rule_diff_arr]: "
-  hnr
-    (master_assn t * id_assn i ii * \<up>(t \<turnstile> xs \<sim> xsi))
-    (diff_arr_lookup_safe xsi ii)
-    (\<lambda>r ri. master_assn t * id_assn r ri)
-    (xs ! i)"
-  unfolding id_rel_def
-  apply(rule hnrI)
-  using lookup_safe by fastforce
+(* lemma merge_or: "a * x * b \<or>\<^sub>A c * x * d = x * (a * b \<or>\<^sub>A c * d)"
+  by (simp add: star_aci(2) star_aci(3) star_or_dist2)
 
-lemma hnr_realize: "
-  hnr
-    (master_assn t * \<up>(t \<turnstile> xs \<sim> xsi))
-    (Diff_Arr.realize xsi)
-    (\<lambda> r ri. master_assn t  * array_assn r ri)
-    xs"
-  unfolding id_rel_def
-  apply(rule hnrI)
-  using realize[of t xs xsi]
-  by(sep_auto simp: cons_post_rule ent_refl_true)
+lemmas merge_ors = merge_or merge_or[of emp] *)
 
-lemma hnr_update[hnr_rule_diff_arr]: "
-  hnr
-    (master_assn t * \<up>(t \<turnstile> xs \<sim> xsi) * id_assn i ii * id_assn v vi)
-    (diff_arr_update_safe xsi ii vi)
-    (\<lambda>xs xsi. \<exists>\<^sub>At'. master_assn t' * 
-              \<up>((\<forall>xs' xsi'. t \<turnstile> xs' \<sim>  xsi' \<longrightarrow> t' \<turnstile> xs' \<sim>  xsi') \<and> t' \<turnstile> xs \<sim> xsi))
-    (xs [i:= v])"
-  unfolding id_rel_def
-  apply(rule hnrI)
+attribute_setup framed =
+    \<open>Scan.succeed (Thm.rule_attribute [] (fn _ => fn thm => @{thm hnr_frame} OF [asm_rl, thm]))\<close>
+    \<open>Add frame to hnr rule\<close>
+
+lemma frame_inference_trivial: "P \<Longrightarrow>\<^sub>A P * emp"
+  by sep_auto
+
+method frame_inference' = rule frame_inference_trivial | frame_inference
+
+lemma move_pure_right: 
+  "a * (b * c) = (a * b) * c" 
+  "NO_MATCH (\<up>(x)) b \<Longrightarrow> \<up>(p) * b = b * \<up>(p)"
+  "NO_MATCH (\<up>(x)) b \<Longrightarrow> a * \<up>(p) * b = a * b * \<up>(p)"
+  by(auto simp: algebra_simps) 
+
+lemma merge_ex: 
+  "(\<exists>\<^sub>Aa _. P a) = (\<exists>\<^sub>Aa. P a)"
+  "(\<exists>\<^sub>A_ a. P a) = (\<exists>\<^sub>Aa. P a)"
+  by simp_all
+
+lemma hnr_pre_cong: "\<Gamma> = \<Gamma>' \<Longrightarrow> hnr \<Gamma> c \<Gamma>'' a = hnr \<Gamma>' c \<Gamma>'' a"
+  by simp
+
+lemma hnr_pre_cong_or_1: "\<lbrakk>\<Gamma>\<^sub>a = \<Gamma>\<^sub>a'; \<Gamma>\<^sub>b = \<Gamma>\<^sub>b'\<rbrakk>
+   \<Longrightarrow> hnr (\<Gamma>\<^sub>a \<or>\<^sub>A \<Gamma>\<^sub>b) c \<Gamma>'' a = hnr (\<Gamma>\<^sub>a' \<or>\<^sub>A \<Gamma>\<^sub>b') c \<Gamma>'' a"
+  by simp
+
+lemma hnr_pre_cong_or_2: "\<lbrakk>\<Gamma>\<^sub>a = \<Gamma>\<^sub>a'; \<Gamma>\<^sub>b = \<Gamma>\<^sub>b'\<rbrakk>
+   \<Longrightarrow> hnr ((\<Gamma>\<^sub>a \<or>\<^sub>A \<Gamma>\<^sub>b) * \<Gamma>\<^sub>c)  c \<Gamma>'' a = hnr ((\<Gamma>\<^sub>a' \<or>\<^sub>A \<Gamma>\<^sub>b') * \<Gamma>\<^sub>c) c \<Gamma>'' a"
+  by simp
+
+lemmas hnr_pre_cong_or = hnr_pre_cong_or_1 hnr_pre_cong_or_2
+
+lemma hnr_pre_cong_or_first_1: "\<lbrakk>\<Gamma>\<^sub>a = \<Gamma>\<^sub>a'\<rbrakk>
+   \<Longrightarrow> hnr (\<Gamma>\<^sub>a \<or>\<^sub>A \<Gamma>\<^sub>b) c \<Gamma>'' a = hnr (\<Gamma>\<^sub>a' \<or>\<^sub>A \<Gamma>\<^sub>b) c \<Gamma>'' a"
+  by simp
+
+lemma hnr_pre_cong_or_first_2: "\<lbrakk>\<Gamma>\<^sub>a = \<Gamma>\<^sub>a'\<rbrakk>
+   \<Longrightarrow> hnr ((\<Gamma>\<^sub>a \<or>\<^sub>A \<Gamma>\<^sub>b) * \<Gamma>\<^sub>c)  c \<Gamma>'' a = hnr ((\<Gamma>\<^sub>a' \<or>\<^sub>A \<Gamma>\<^sub>b) * \<Gamma>\<^sub>c) c \<Gamma>'' a"
+  by simp
+
+lemmas hnr_pre_cong_or_first = hnr_pre_cong_or_first_1 hnr_pre_cong_or_first_2
+
+lemma hnr_extract_pure_1:
+  assumes
+    "p \<Longrightarrow> hnr \<Gamma> c \<Gamma>' a"
+  shows 
+    "hnr (\<Gamma> * \<up>(p)) c \<Gamma>' a"
+  using assms 
+  unfolding hnr_def
+  apply(cases p) 
+  by auto
+
+lemma hnr_extract_pure_2:
+  assumes
+    "p \<Longrightarrow> hnr emp c \<Gamma>' a"
+  shows 
+    "hnr (\<up>(p)) c \<Gamma>' a"
+  using assms 
+  unfolding hnr_def
+  apply(cases p) 
+  by auto
+
+lemma hnr_exE:
+   assumes
+   "\<And>x. hnr (P x) c (\<Gamma>' x) a"
+  shows 
+    "hnr (\<exists>\<^sub>Ax. P x) c (\<lambda>u v. \<exists>\<^sub>Ax. \<Gamma>' x u v) a"
+  using assms
+  unfolding hnr_def
   apply(sep_auto)
   apply(rule cons_post_rule)
-  apply(rule fi_rule[OF update_safe])
-  by sep_auto+
+   apply blast 
+  by solve_entails
+
+lemmas hnr_extract_pure = hnr_extract_pure_1 hnr_extract_pure_2 hnr_exE
+
+lemma prepare_frame_1:
+  assumes
+    "emp * P * emp \<Longrightarrow>\<^sub>A emp * Q * F"
+  shows
+    "P \<Longrightarrow>\<^sub>A Q * F"
+  using assms
+  by sep_auto
+
+lemma frame_no_match: 
+  assumes
+    "Ps1 * (P * Ps2) \<Longrightarrow>\<^sub>A Qs * Q * F"
+  shows
+    "Ps1 * P * Ps2 \<Longrightarrow>\<^sub>A Qs * Q * F"
+  using assms
+  by (simp add: mult.assoc)
+
+lemma frame_match_pure:
+  assumes
+    "P"
+    "Ps \<Longrightarrow>\<^sub>A Qs * F"
+  shows
+    "Ps \<Longrightarrow>\<^sub>A Qs * \<up>(P) * F"
+  using assms
+  by simp
+
+lemma frame_match:
+  assumes
+    "Ps1 * Ps2 \<Longrightarrow>\<^sub>A Qs * F"
+  shows
+    "Ps1 * P * Ps2 \<Longrightarrow>\<^sub>A Qs * P * F"
+  using assms
+  by (metis assn_aci(10) fr_refl)
+
+lemma frame_match_emp:
+   assumes
+    "Ps \<Longrightarrow>\<^sub>A Qs * F"
+  shows
+    "Ps \<Longrightarrow>\<^sub>A Qs * emp * F"
+  using assms
+  by sep_auto
+
+lemma frame_done: "F * emp \<Longrightarrow>\<^sub>A emp * F" 
+  by sep_auto
+
+lemma ex_assn_move_in:
+  "\<And>Q R. (\<exists>\<^sub>Ax. Q x * R) = (\<exists>\<^sub>Ax. Q x) * R"
+  "\<And>Q R. (\<exists>\<^sub>Ax. Q * R x) = Q * (\<exists>\<^sub>Ax. R x)"
+  "(\<exists>\<^sub>Ax. Q x * R x) = (\<exists>\<^sub>Ax. Q x) * (\<exists>\<^sub>Ax. R x)" 
+   apply sep_auto
+   apply sep_auto
+  (* TODO Important: How to have rule just in one direction? *)
+  sorry
+
+lemma hnr_or_match_1:
+  assumes
+    "hnr ((As1 * As2 \<or>\<^sub>A Bs1 * Bs2) * (A * Cs)) fi \<Gamma>' f"
+  shows
+    "hnr ((As1 * A * As2 \<or>\<^sub>A Bs1 * A * Bs2) * Cs) fi \<Gamma>' f"
+  apply(rule hnrI)
+  using 
+    assms[THEN hnrD]
+  by (metis star_aci(3) star_assoc star_or_dist2)
+
+lemma hnr_or_match_2:
+  assumes
+    "hnr ((As1 * As2 \<or>\<^sub>A Bs1 * Bs2) * ((\<exists>\<^sub>A x. A x) * Cs)) fi \<Gamma>' f"
+  shows
+    "hnr ((As1 * (\<exists>\<^sub>A x. A x) * As2 \<or>\<^sub>A Bs1 * A x * Bs2) * Cs) fi \<Gamma>' f"
+  apply(rule hnrI)
+  using 
+    assms[THEN hnrD]
+  by (smt (verit, ccfv_threshold) assn_aci(10) assn_times_comm cons_pre_rule ent_disjE ent_disjI1_direct ent_disjI2' fr_refl star_or_dist1 triv_exI)
+
+lemma hnr_or_match_3:
+  assumes
+    "hnr ((As1 * As2 \<or>\<^sub>A Bs1 * Bs2) * ((\<exists>\<^sub>A x. A x) * Cs)) fi \<Gamma>' f"
+  shows
+    "hnr ((As1 * A x * As2 \<or>\<^sub>A Bs1 * (\<exists>\<^sub>A x. A x) * Bs2) * Cs) fi \<Gamma>' f"
+  apply(rule hnrI)
+  using 
+    assms[THEN hnrD]
+  sorry
+  (* TODO: 
+  by (smt (verit, ccfv_SIG) SLN_right ac_operator.right_commute cons_pre_rule ent_disjE ent_disjI1_direct ent_disjI2_direct ent_frame_fwd ent_star_mono fr_refl keep_drop_2 mult.ac_operator_axioms triv_exI)
+  *)
+
+lemma hnr_or_match_4:
+  assumes
+    "hnr Cs fi \<Gamma>' f"
+  shows
+    "hnr ((\<up>c * emp \<or>\<^sub>A \<up>(\<not>c) * emp) * Cs) fi \<Gamma>' f"
+  apply(rule hnrI)
+  using 
+    assms[THEN hnrD]
+  by simp
+
+lemmas hnr_or_match = hnr_or_match_1 hnr_or_match_2 hnr_or_match_3 hnr_or_match_4
+
+lemma hnr_or_prepare:
+  assumes
+    "hnr ((As * emp \<or>\<^sub>A Bs * emp) * Cs) fi \<Gamma>' f"
+  shows
+    "hnr ((As \<or>\<^sub>A Bs) * Cs) fi \<Gamma>' f"
+  apply(rule hnrI)
+  using 
+    assms[THEN hnrD]
+  by simp
+
+lemma hnr_or_no_match_1:
+  assumes
+    "hnr ((As1 * (A * As2) \<or>\<^sub>A Bs1 * B * Bs2) * Cs) fi \<Gamma>' f"
+  shows
+    "hnr ((As1 * A * As2 \<or>\<^sub>A Bs1 * B * Bs2) * Cs) fi \<Gamma>' f"
+  apply(rule hnrI)
+  using 
+    assms[THEN hnrD]
+  by (simp add: mult.left_assoc)
+
+lemma id: "A = A"
+  by simp
+
+(* lemma frame_no_match: 
+  assumes
+    "Ps1 * (P * Ps2) \<Longrightarrow>\<^sub>A Qs * Q * F"
+  shows
+    "Ps1 * P * Ps2 \<Longrightarrow>\<^sub>A Qs * Q * F"
+  using assms
+  by (simp add: mult.assoc) *)
+
+method normalize_hnr_pre = simp(no_asm) named_ss HOL_basic_ss_nomatch:
+    move_pure_right assn_one_left mult_1_right[where 'a=assn] 
+    merge_pure_star[symmetric] ex_assn_move_out pure_true
+  cong: hnr_pre_cong
+
+find_theorems "\<not>_" "(\<noteq>)"
+
+method normalize_or_hnr_pre uses cong = simp(no_asm) named_ss HOL_basic_ss_nomatch:
+    assn_one_left mult_1_right[where 'a=assn] (* TODO Name: *) move_pure_right(1)
+    merge_pure_star[symmetric] ex_assn_move_in pure_true merge_ex
+  cong: cong
+
+method hnr_or_no_match = then_else 
+  \<open>rule hnr_or_no_match_1\<close> 
+  \<open>rule id\<close> 
+  \<open>normalize_or_hnr_pre cong: hnr_pre_cong_or_first, rule hnr_or_prepare\<close>
+
+
+lemma ex_or1: "(\<exists>\<^sub>Aa b. P a  \<or>\<^sub>A P b) \<Longrightarrow>\<^sub>A (\<exists>\<^sub>Aa. P a)"
+  by (simp add: ent_disjE ent_ex_preI)
+ 
+lemma ex_or2: "(\<exists>\<^sub>Aa. P a) \<Longrightarrow>\<^sub>A (\<exists>\<^sub>Aa b. P a  \<or>\<^sub>A P b)"
+  by (meson ent_disjI1_direct ent_ex_postI ent_ex_preI)
+
+lemma ex_or: "(\<exists>\<^sub>Aa b. P a  \<or>\<^sub>A P b) = (\<exists>\<^sub>Aa. P a)"
+  apply(rule ent_iffI)
+  using ex_or1 ex_or2 by auto
+
+lemma ex_or_x: "(\<exists>\<^sub>Aa. P a \<or>\<^sub>A P b) \<Longrightarrow>\<^sub>A (\<exists>\<^sub>Aa. P a)"
+  by (simp add: ent_disjE ent_ex_preI)
+
+(* 
+lemma hnr_if: 
+  assumes
+    "hnr \<Gamma> ai \<Gamma>\<^sub>a a"
+    "hnr \<Gamma> bi \<Gamma>\<^sub>b b"
+  shows 
+    "hnr 
+      \<Gamma> 
+      (if c then ai else bi) 
+      (\<lambda>a r. \<Gamma>\<^sub>a a r * \<up> c \<or>\<^sub>A \<Gamma>\<^sub>b a r * \<up>(\<not>c)) 
+      (if c then a else b)" 
+  supply[sep_heap_rules] = assms[THEN hnrD]
+  apply(rule hnrI)
+  by(sep_auto simp: ent_star_mono)*)
+
+(* lemma merge_if_1:
+  assumes 
+    "c" 
+    "hnr \<Gamma>\<^sub>a x \<Gamma> xi" 
+  shows 
+   "hnr (\<Gamma>\<^sub>a * \<up> c \<or>\<^sub>A \<Gamma>\<^sub>b * \<up>(\<not>c)) x \<Gamma> xi" 
+  using assms
+  by sep_auto
+
+lemma merge_if_2:
+  assumes 
+    "\<not>c" 
+    "hnr \<Gamma>\<^sub>b x \<Gamma> xi" 
+   shows 
+    "hnr (\<Gamma>\<^sub>a * \<up> c \<or>\<^sub>A \<Gamma>\<^sub>b * \<up>(\<not>c)) x  \<Gamma> xi"
+  using assms
+  by sep_auto
+
+lemma merge_if_fallback:
+  assumes 
+    "hnr true x \<Gamma> xi" 
+   shows 
+    "hnr (\<Gamma>\<^sub>a \<or>\<^sub>A \<Gamma>\<^sub>b) x  \<Gamma> xi"
+  apply(rule hnrI)
+  using assms[THEN hnrD]
+  using cons_pre_rule ent_true by blast *)
+
+(* Steps for merging: 
+  1. Simply or [merge_or] and bring \<exists>. to the outside (if possible combine \<exists> already)
+  2. Match real t with \<exists>. to \<exists>.
+  3. Rest: c \<rightarrow> X * \<not>c \<rightarrow> Y (Does it work like this?)
+*)
+
+
+
+(* lemma merge_if_1:
+  assumes 
+    "hnr (\<exists>\<^sub>At'. master_assn t' * \<up>(t' \<turnstile> xs \<sim> xsi)) x \<Gamma> xi" 
+   shows 
+    "hnr (master_assn t * \<up>(t \<turnstile> xs \<sim> xsi) \<or>\<^sub>A (\<exists>\<^sub>At'. master_assn t' * \<up>(t' \<turnstile> xs \<sim> xsi))) x  \<Gamma> xi"
+  apply(rule hnrI)
+  apply(rule split_rule)
+  using cons_pre_rule assms[THEN hnrD] apply fastforce
+  using assms[THEN hnrD] by simp
+
+(* 
+   hnr (master_assn t * \<up> (t \<turnstile> t1 \<sim> xia) * emp * \<up> True \<or>\<^sub>A
+                (\<exists>\<^sub>At'.
+                    master_assn t' *
+                    \<up> ((\<forall>xs' xsi'. t \<turnstile> xs' \<sim> xsi' \<longrightarrow> t' \<turnstile> xs' \<sim> xsi') \<and> t' \<turnstile> t1 \<sim> xia)) *
+                emp *
+                \<up> (\<not> True))
+*)
+
+lemma merge_if_2:
+  assumes 
+    "hnr ((\<exists>\<^sub>At'. master_assn t' * \<up>(t' \<turnstile> xs \<sim> xsi))) x \<Gamma> xi" 
+   shows 
+    "hnr (master_assn t * \<up>(t \<turnstile> xs \<sim> xsi) * emp \<or>\<^sub>A 
+          (\<exists>\<^sub>At'. master_assn t' * \<up>(t' \<turnstile> xs \<sim> xsi))) x  \<Gamma> xi"
+  apply(rule hnrI)
+  apply(rule split_rule)
+  using cons_pre_rule assms[THEN hnrD]
+  apply fastforce
+  using assms[THEN hnrD] cons_pre_rule by sep_auto
+
+find_theorems "(\<Longrightarrow>\<^sub>A)" "\<exists>\<^sub>A _ . _"
+
+
+
+lemma t: assumes "P" shows "P" using assms by simp
+
+lemma wtf_1: "fold_assn t \<Longrightarrow>\<^sub>A \<exists>\<^sub>Ax. fold_assn x" 
+  by simp
+
+lemma wtf_2: "master_assn t = master_assn t"
+  by auto
+
+lemma wtf_5: "master_assn t \<Longrightarrow>\<^sub>A master_assn t"
+  by auto
+
+lemma wtf_6: "master_assn t \<Longrightarrow>\<^sub>A \<exists>\<^sub>Ax. master_assn t"
+  by auto
+
+lemma wtf_8: assumes "master_assn t \<Longrightarrow>\<^sub>A \<exists>\<^sub>Ax. master_assn x"
+  shows "master_assn t \<Longrightarrow>\<^sub>A \<exists>\<^sub>Ax. master_assn x"
+  using assms
+  sorry
+
+lemma wtf_7: "master_assn t \<Longrightarrow>\<^sub>A \<exists>\<^sub>Ax. master_assn x"
+  using triv_exI[of master_assn t]
+  sorry
+
+lemma merge_or_master_assn_1_1:
+  assumes 
+    "hnr (\<exists>\<^sub>At'. master_assn t') x \<Gamma> xi"
+   shows 
+    "hnr (master_assn t \<or>\<^sub>A (\<exists>\<^sub>At'. master_assn t')) x \<Gamma> xi"
+  apply(rule hnrI)
+  apply(rule split_rule)
+  using cons_pre_rule[of "master_assn t" "\<exists>\<^sub>At'. master_assn t'" x  "(\<lambda>b. \<Gamma> xi b * true)"] assms[THEN hnrD] 
+  using wtf_7[of t]
+   apply blast
+  using assms[THEN hnrD]
+  apply blast
+  sorry
+
+lemma merge_or_master_assn_1:
+  assumes 
+    "hnr (\<exists>\<^sub>At'. master_assn t') x \<Gamma> xi"
+   shows 
+    "hnr (\<exists>\<^sub>At'. master_assn t \<or>\<^sub>A master_assn t') x  \<Gamma> xi"
+  apply(rule hnrI)
+  using assms[THEN hnrD]
+  apply sep_auto
+  sorry *)
+  
+method frame_norm_assoc = (simp only: mult.left_assoc[where 'a=assn])?
+
+method frame_prepare = rule prepare_frame_1, frame_norm_assoc
+
+method frame_try_match = then_else 
+  \<open>rule frame_match_pure, assumption | rule frame_match frame_match_emp\<close> 
+  \<open>frame_norm_assoc\<close> 
+  \<open>rule frame_no_match, frame_try_match\<close>
+
+method or_match = 
+  (normalize_or_hnr_pre cong: hnr_pre_cong_or, rule hnr_or_prepare), 
+  (rule hnr_or_match | hnr_or_no_match) 
+
+method frame_done = simp only: assn_one_left mult_1_right[where 'a=assn], rule ent_refl  
+
+method frame_inference_2 = frame_prepare, frame_try_match+, frame_done
+
+method frame_inference_2_dbg = frame_prepare, (frame_try_match+)?, frame_done?
+
+experiment
+begin
+
+schematic_goal 
+  fixes a b c d::assn
+  shows "a * b * c * d \<Longrightarrow>\<^sub>A a * c * ?F"
+    apply frame_inference_2
+  done
+
+schematic_goal 
+  fixes a b c d::assn
+  shows "a * b * c * d \<Longrightarrow>\<^sub>A emp * ?F"
+   apply frame_inference_2
+  done
+
+schematic_goal 
+  fixes a b c d::assn
+  shows "emp \<Longrightarrow>\<^sub>A emp * ?F"
+   apply frame_inference_2
+  done
+
+schematic_goal 
+  fixes a b c d::assn
+  shows "a * b * c * d \<Longrightarrow>\<^sub>A b * d * ?F"
+   apply frame_inference_2
+  done
+
+schematic_goal 
+  shows "a * \<up>(b) * c * d \<Longrightarrow>\<^sub>A \<up>(b) * d * ?F"
+   apply frame_inference_2
+  done
+end
+
+method hnr_extract_pure methods post_processing = 
+  normalize_hnr_pre?, ((rule hnr_extract_pure)+)?, post_processing?
+
+method hnr_rule uses rule_set = 
+  (rule rule_set[framed] hnr_copy[framed], frame_inference_2) | rule hnr_rule hnr_return
+
+method hnr methods assumption_processing uses rule_set =
+  (hnr_extract_pure assumption_processing, ((hnr_rule rule_set: rule_set) | keep_drop))+
 
 end
