Hnr_Array.thy
@@ -1,0 +1,53 @@
+theory Hnr_Array
+  imports Hnr Array_Safe
+begin
+
+named_theorems hnr_rule_arr
+
+lemma hnr_new: 
+  "hnr 
+    (id_assn n ni * id_assn x xi) 
+    (Array.new ni xi) 
+    (\<lambda>xs xsi. xsi \<mapsto>\<^sub>a xs * id_assn n ni * id_assn x xi) 
+    (replicate n x)"
+  unfolding id_rel_def
+  apply(rule hnrI)
+  by sep_auto
+
+lemma hnr_array_of_list: 
+  "hnr 
+    emp
+    (Array.of_list xs) 
+    (\<lambda>xs xsi. xsi \<mapsto>\<^sub>a xs) 
+    xs"
+  unfolding id_rel_def
+  apply(rule hnrI)
+  by sep_auto
+
+lemma hnr_array_nth [hnr_rule_arr]: "
+    hnr
+     (xsi \<mapsto>\<^sub>a xs * id_assn i ii)
+     (array_nth_safe xsi ii) 
+     (\<lambda> r ri. xsi \<mapsto>\<^sub>a xs * id_assn r ri) 
+     (xs ! i)"
+  unfolding id_rel_def
+  apply(rule hnrI)
+  by sep_auto
+
+lemma hnr_array_update [hnr_rule_arr]: "
+    hnr 
+      (xsi \<mapsto>\<^sub>a xs * id_assn i ii * id_assn v vi) 
+      (array_update_safe ii vi xsi) 
+      array_assn
+      (xs [i:= v])"
+  unfolding id_rel_def
+  apply(rule hnrI)
+  by sep_auto
+
+lemma hnr_copy_arr [hnr_rule_arr]:
+  "hnr (array_assn x xi) (return xi) array_assn x"
+  using hnr_pass by fastforce
+
+method hnr_arr = hnr - rule_set: hnr_rule_arr
+
+end
