Hnr_Diff_Arr.thy
@@ -1,0 +1,80 @@
+theory Hnr_Diff_Arr
+  imports Hnr Diff_Arr_Safe
+begin
+
+named_theorems hnr_rule_diff_arr
+
+lemma hnr_copy_diff_arr [hnr_rule_diff_arr]:
+  "hnr (master_assn t * \<up>(t \<turnstile> x \<sim> xi)) (return xi) (\<lambda>x xi. master_assn t * \<up>(t \<turnstile> x \<sim> xi)) x"
+  apply(rule hnrI)
+  by sep_auto
+
+lemma hnr_from_array: 
+  "hnr 
+    (array_assn xs xsi)
+    (Diff_Arr.from_array xsi)
+    (\<lambda>xs xsi. \<exists>\<^sub>At. master_assn t * \<up>(t \<turnstile> xs \<sim> xsi))
+    xs
+  "
+  apply(rule hnrI)
+  using ent_refl_true fi_rule from_array by blast
+
+lemma hnr_from_list: 
+  "hnr 
+    emp
+    (Diff_Arr.from_list xs)
+    (\<lambda>xs xsi. \<exists>\<^sub>At. master_assn t * \<up>(t \<turnstile> xs \<sim> xsi))
+    xs
+  "
+  apply(rule hnrI)
+  using ent_refl_true fi_rule from_list by blast
+
+lemma hnr_lookup[hnr_rule_diff_arr]: "
+  hnr
+    (master_assn t * id_assn i ii * \<up>(t \<turnstile> xs \<sim> xsi))
+    (diff_arr_lookup_safe xsi ii)
+    (\<lambda>r ri. master_assn t * id_assn r ri)
+    (xs ! i)"
+  unfolding id_rel_def
+  apply(rule hnrI)
+  using lookup_safe by fastforce
+
+lemma hnr_realize: "
+  hnr
+    (master_assn t * \<up>(t \<turnstile> xs \<sim> xsi))
+    (Diff_Arr.realize xsi)
+    (\<lambda> r ri. master_assn t  * array_assn r ri)
+    xs"
+  unfolding id_rel_def
+  apply(rule hnrI)
+  using realize[of t xs xsi]
+  by(sep_auto simp: cons_post_rule ent_refl_true)
+
+lemma hnr_update[hnr_rule_diff_arr]: "
+  hnr
+    (master_assn t * \<up>(t \<turnstile> xs \<sim> xsi) * id_assn i ii * id_assn v vi)
+    (diff_arr_update_safe xsi ii vi)
+    (\<lambda>xs xsi. \<exists>\<^sub>At'. master_assn t' * 
+              \<up>((\<forall>xs' xsi'. t \<turnstile> xs' \<sim>  xsi' \<longrightarrow> t' \<turnstile> xs' \<sim>  xsi') \<and> t' \<turnstile> xs \<sim> xsi))
+    (xs [i:= v])"
+  unfolding id_rel_def
+  apply(rule hnrI)
+  apply(sep_auto)
+  apply(rule cons_post_rule)
+  apply(rule fi_rule[OF update_safe])
+  by sep_auto+  
+
+lemma transfer_diff_arr_rel:
+  assumes 
+    "t \<turnstile> xs \<sim> xsi" 
+    "\<forall>xs xsi. t \<turnstile> xs \<sim> xsi \<longrightarrow> t' \<turnstile> xs \<sim> xsi"
+  shows 
+    "t' \<turnstile> xs \<sim> xsi"
+  using assms by blast
+
+method hnr_transfer_diff_arr_rel = 
+  ((drule(1) transfer_diff_arr_rel)+)?, (thin_tac "\<forall>xs' xsi'. _ \<turnstile> xs' \<sim> xsi' \<longrightarrow> _ \<turnstile> xs' \<sim> xsi'")
+
+method hnr_diff_arr = hnr hnr_transfer_diff_arr_rel rule_set: hnr_rule_diff_arr
+
+end
