Test_Diff_Arr.thy
@@ -1,0 +1,23 @@
+theory Test_Diff_Arr
+  imports Diff_Arr
+begin
+
+definition create_diff_arr where
+  "create_diff_arr n x = do {
+    a \<leftarrow> Array.new n x;
+    Diff_Arr.from_array a
+  }"
+
+definition test where "test = do {
+  r \<leftarrow> create_diff_arr 3 (5::nat);
+  y  \<leftarrow> Diff_Arr.update r 1 (7::nat);
+  y' \<leftarrow> Diff_Arr.update r 1 (8::nat);
+  x \<leftarrow> Diff_Arr.lookup y 1;
+  return x
+}"
+
+ML_val \<open>@{code test} ()\<close>
+
+export_code test in SML_imp module_name foo
+
+end
