Test_Hnr.thy
@@ -1,0 +1,182 @@
+theory Test_Hnr
+  imports Hnr_Diff_Arr Hnr_Array "HOL-Library.Code_Target_Nat" 
+begin
+
+definition test1 where
+  "test1 xs = 
+    (let c1 = (let x = 1 in x); c2 = 2; c3 = 3; t1 = xs[c1 := c2]; t2 = t1[c1 := c3]; t3 = t2 ! c2 in t3)"
+
+definition test2 where
+  "test2 xs = 
+    (let c1 = 1; t1 = xs[c1 := c1] in t1)"
+
+definition test2_1 where
+  "test2_1 xs = 
+    (let c1 = 1; t1 = xs[c1 := c1] in (c1, t1))"
+
+definition test2_2 where
+  "test2_2 xs = 
+    (let c1 = 1; t1 = xs; t2 = xs[c1 := c1] in (t1, t2))"
+
+definition test2_3 where
+  "test2_3 xs = 
+    (let c1 = 1; c2 = 2 in (c1, c2))"
+
+definition test3 where
+  "test3 xs = 
+    (let c1 = 1; t1 = xs[c1 := c1]; t2 = xs ! c1 in t1)"
+
+definition test4 where
+  "test4 xs =
+    (let c1 = 1; t1 = if xs = [] then xs else let t2 = xs[c1 := c1] in t2 in t1)"
+
+definition test4_2 where
+  "test4_2 xs =
+    (let c1 = 1; t1 = if xs = [] then xs else let t1 = xs[c1 := c1]; t2 = t1[c1:= c1] in t2 in t1)"
+
+definition test4_3 where
+  "test4_3 xs =
+    (let c1 = 1; t1 = if xs = [] then let c2 = 2; t1 = xs[c2 := c2]; t2 = t1[c2:= c2] in xs else let t1 = xs[c1 := c1]; t2 = t1[c1:= c1] in t2 in t1)"
+
+(* TODO: What to do if the bool depends on local variables? *)
+definition test5 where
+  "test5 xs = 
+    (let c1 = 1; t1 = if c1 = 0 then xs else xs[c1 := c1] in t1)"
+
+(* TODO: I need this form but need to find a way for comparisons *)
+definition test5_1 where
+  "test5_1 xs = 
+    (let c1 = 1; b = (c1 = c1); t1 = if b then xs else xs[c1 := c1] in t1)"
+
+definition test6 where
+  "test6 xs = 
+    (let c1 = 1; c2 = 2; t1 = if xs = [] then xs[c2 := c2] else xs[c1 := c1] in t1)"
+
+definition test7 where
+  "test7 xs = 
+    (let c1 = 1; c2 = 2; t1 = if xs = [] then let t2 = xs[c2 := c2]; t3 = xs[c1 := c1] in t3 else let t2 = xs[c1 := c1]; t3 = xs[c2 := c1] in t3 in t1)"
+
+
+schematic_goal "hnr (array_assn xs xsi) (?c :: ?'a Heap) ?\<Gamma>' (test1 xs)"
+  unfolding test1_def 
+  apply hnr_arr
+  done
+
+schematic_goal "hnr (array_assn xs xsi) (?c :: ?'a Heap) ?\<Gamma>' (test2 xs)"
+  unfolding test2_def 
+  apply hnr_arr
+  done  
+
+schematic_goal "hnr (array_assn xs xsi) (?c :: ?'a Heap) ?\<Gamma>' (test2_1 xs)"
+  unfolding test2_1_def 
+  apply hnr_arr
+  done  
+
+schematic_goal "hnr (array_assn xs xsi) (?c :: ?'a Heap) ?\<Gamma>' (test2_3 xs)"
+  unfolding test2_3_def 
+  apply hnr_arr
+  done  
+
+(* Can't work, not linear! *)
+schematic_goal "hnr (array_assn xs xsi) (?c :: ?'a Heap) ?\<Gamma>' (test3 xs)"
+  unfolding test3_def 
+  apply hnr_arr
+  sorry
+
+schematic_goal "hnr (master_assn t * \<up>(t \<turnstile> xs \<sim> xsi)) (?c :: ?'a Heap) ?\<Gamma>' (test1 xs)"
+  unfolding test1_def
+  apply hnr_diff_arr
+  done
+
+schematic_goal "hnr (master_assn t * \<up>(t \<turnstile> xs \<sim> xsi)) (?c :: ?'a Heap) ?\<Gamma>' (test2 xs)"
+  unfolding test2_def
+  apply hnr_diff_arr
+  done
+
+schematic_goal "hnr (master_assn t * \<up>(t \<turnstile> xs \<sim> xsi)) (?c :: ?'a Heap) ?\<Gamma>' (test2_1 xs)"
+  unfolding test2_1_def
+  apply hnr_diff_arr
+  done
+
+schematic_goal "hnr (master_assn t * \<up>(t \<turnstile> xs \<sim> xsi)) (?c :: ?'a Heap) ?\<Gamma>' (test2_2 xs)"
+  unfolding test2_2_def
+  apply hnr_diff_arr
+  done
+
+schematic_goal "hnr (master_assn t * \<up>(t \<turnstile> xs \<sim> xsi)) (?c :: ?'a Heap) ?\<Gamma>' (test2_3 xs)"
+  unfolding test2_3_def
+  apply hnr_diff_arr
+  done
+
+schematic_goal "hnr (master_assn t * \<up>(t \<turnstile> xs \<sim> xsi)) (?c xsi :: ?'a Heap) (?\<Gamma>' xsi xs) (test3 xs)"
+  unfolding test3_def
+  apply hnr_diff_arr
+  done  
+
+schematic_goal "hnr (master_assn t * \<up>(t \<turnstile> xs \<sim> xsi)) (?c xsi :: ?'a Heap) (?\<Gamma>' xsi xs) (test4 xs)"
+  unfolding test4_def
+  sorry
+  (* apply hnr_diff_arr
+     apply (rule hnr_if)
+      apply hnr_diff_arr
+  subgoal sorry
+  subgoal 
+    apply(rule merge_if_2)
+    apply hnr_diff_arr
+  sorry *)
+
+lemma cool_rule: "(\<exists>\<^sub>A x y. P x) = (\<exists>\<^sub>A x. P x)"
+  by simp
+
+schematic_goal "hnr (master_assn t * \<up>(t \<turnstile> xs \<sim> xsi)) (?c xsi :: ?'a Heap) (?\<Gamma>' xsi xs) (test4_2 xs)"
+  unfolding test4_2_def
+  apply hnr_diff_arr
+  apply or_match+   
+  subgoal sorry       
+  subgoal sorry
+  subgoal sorry
+  sorry
+  (* apply hnr_diff_arr
+
+     apply (rule hnr_if)
+      apply hnr_diff_arr
+  apply simp
+    apply(rule merge_if_2)
+    apply hnr_diff_arr
+  done *)
+
+schematic_goal "hnr (master_assn t * \<up>(t \<turnstile> xs \<sim> xsi)) (?c xsi :: ?'a Heap) (?\<Gamma>' xsi xs) (test4_3 xs)"
+  unfolding test4_3_def
+  apply hnr_diff_arr
+  apply or_match+
+  subgoal sorry       
+  subgoal sorry
+  subgoal sorry
+  sorry
+
+schematic_goal "hnr (master_assn t * \<up>(t \<turnstile> xs \<sim> xsi)) (?c xsi :: ?'a Heap) (?\<Gamma>' xsi xs) (test5_1 xs)"
+  unfolding test5_1_def
+  
+  sorry
+
+schematic_goal "hnr (master_assn t * \<up>(t \<turnstile> xs \<sim> xsi)) (?c xsi :: ?'a Heap) (?\<Gamma>' xsi xs) (test7 xs)"
+  unfolding test7_def
+  apply hnr_diff_arr
+  apply or_match+
+  subgoal sorry
+  subgoal sorry
+  subgoal sorry
+  subgoal sorry
+  sorry
+
+(* 
+  Questions/Notes: 
+  - Wouldn't it be more useful to always build up the master_assn instead of using existensials?
+  - How to integrate standard operations like + and -? Bool ops? Simple function call? 
+  - How to integrate Annotations?
+*)
+
+
+export_code array_nth_safe array_update_safe in SML_imp
+
+end
